Prove LR and RL lemmas

src/drf/SmallStep.v
@@ -282,3 +282,298 @@ Proof.
   setoid_rewrite Cell.bot_get in PROMISES0. done.
 Qed.
 
+Inductive nonpromise c l f t msg :=
+| nonpromise_intro
+    (GET: Memory.get l t c.(Configuration.memory) = Some (f, msg))
+    (NONPROMISE: forall tid, ~ Threads.is_promised tid l t c.(Configuration.threads))
+.
+
+Lemma writing_small_step_nonpromise_forward
+      withprm tid e c1 c2 loc from to val released ord
+      (WF: Configuration.wf c1)
+      (STEP: small_step withprm tid e c1 c2)
+      (WRITING: ThreadEvent.is_writing e = Some (loc, from, to, val, released, ord)):
+  forall l f t msg
+    (NP: nonpromise c1 l f t msg),
+    nonpromise c2 l f t msg.
+Proof.
+  inv STEP. inv STEP0; inv STEP; inv WRITING.
+  - inv LOCAL. inv WRITE. inv PROMISE.
+    { i. inv NP. econs; s.
+      - erewrite Memory.add_o; eauto. condtac; ss.
+        des. subst. exploit Memory.add_get0; eauto. congr.
+      - ii. inv H. revert TID0. rewrite IdentMap.gsspec. condtac.
+        + i. inv TID0. apply inj_pair2 in H1. subst. ss.
+          revert PROMISES0. erewrite Memory.remove_o; eauto. condtac; ss.
+          erewrite Memory.add_o; eauto. condtac; ss. i.
+          eapply NONPROMISE. econs; eauto.
+        + i. eapply NONPROMISE. econs; eauto.
+    }
+    { i. inv NP. econs; s.
+      - erewrite Memory.split_o; eauto. condtac; ss.
+        { des. subst. exploit Memory.split_get0; eauto. i. des. congr. }
+        condtac; ss. guardH o. des. subst.
+        exfalso. eapply NONPROMISE. econs; eauto.
+        hexploit Memory.split_get0; try exact PROMISES; eauto. i. des. eauto.
+      - ii. inv H. revert TID0. rewrite IdentMap.gsspec. condtac.
+        + i. inv TID0. apply inj_pair2 in H1. subst. ss.
+          revert PROMISES0. erewrite Memory.remove_o; eauto. condtac; ss.
+          erewrite Memory.split_o; eauto. repeat condtac; ss.
+          * guardH o. guardH o0. i. des. inv PROMISES0.
+            eapply NONPROMISE. econs; eauto.
+            hexploit Memory.split_get0; try exact PROMISES; eauto. i. des. eauto.
+          * i. eapply NONPROMISE. econs; eauto.
+        + i. eapply NONPROMISE. econs; eauto.
+    }
+    { i. inv NP. econs; s.
+      - erewrite Memory.lower_o; eauto. condtac; ss.
+        des. subst. exfalso. eapply NONPROMISE. econs; eauto.
+        hexploit Memory.lower_get0; try exact PROMISES; eauto.
+      - ii. inv H. revert TID0. rewrite IdentMap.gsspec. condtac.
+        + i. inv TID0. apply inj_pair2 in H1. subst. ss.
+          revert PROMISES0. erewrite Memory.remove_o; eauto. condtac; ss.
+          erewrite Memory.lower_o; eauto. condtac; ss.
+          guardH o. guardH o0. i. des. inv PROMISES0.
+          eapply NONPROMISE. econs; eauto.
+        + i. eapply NONPROMISE. econs; eauto.
+    }
+  - inv LOCAL1. clear GET.
+    inv LOCAL2. inv WRITE. inv PROMISE.
+    { i. inv NP. econs; s.
+      - erewrite Memory.add_o; eauto. condtac; ss.
+        des. subst. exploit Memory.add_get0; eauto. congr.
+      - ii. inv H. revert TID0. rewrite IdentMap.gsspec. condtac.
+        + i. inv TID0. apply inj_pair2 in H1. subst. ss.
+          revert PROMISES0. erewrite Memory.remove_o; eauto. condtac; ss.
+          erewrite Memory.add_o; eauto. condtac; ss. i.
+          eapply NONPROMISE. econs; eauto.
+        + i. eapply NONPROMISE. econs; eauto.
+    }
+    { i. inv NP. econs; s.
+      - erewrite Memory.split_o; eauto. condtac; ss.
+        { des. subst. exploit Memory.split_get0; eauto. i. des. congr. }
+        condtac; ss. guardH o. des. subst.
+        exfalso. eapply NONPROMISE. econs; eauto.
+        hexploit Memory.split_get0; try exact PROMISES; eauto. i. des. eauto.
+      - ii. inv H. revert TID0. rewrite IdentMap.gsspec. condtac.
+        + i. inv TID0. apply inj_pair2 in H1. subst. ss.
+          revert PROMISES0. erewrite Memory.remove_o; eauto. condtac; ss.
+          erewrite Memory.split_o; eauto. repeat condtac; ss.
+          * guardH o. guardH o0. i. des. inv PROMISES0.
+            eapply NONPROMISE. econs; eauto.
+            hexploit Memory.split_get0; try exact PROMISES; eauto. i. des. eauto.
+          * i. eapply NONPROMISE. econs; eauto.
+        + i. eapply NONPROMISE. econs; eauto.
+    }
+    { i. inv NP. econs; s.
+      - erewrite Memory.lower_o; eauto. condtac; ss.
+        des. subst. exfalso. eapply NONPROMISE. econs; eauto.
+        hexploit Memory.lower_get0; try exact PROMISES; eauto.
+      - ii. inv H. revert TID0. rewrite IdentMap.gsspec. condtac.
+        + i. inv TID0. apply inj_pair2 in H1. subst. ss.
+          revert PROMISES0. erewrite Memory.remove_o; eauto. condtac; ss.
+          erewrite Memory.lower_o; eauto. condtac; ss.
+          guardH o. guardH o0. i. des. inv PROMISES0.
+          eapply NONPROMISE. econs; eauto.
+        + i. eapply NONPROMISE. econs; eauto.
+    }
+Qed.
+
+Lemma writing_small_step_nonpromise_new
+      withprm tid e c1 c2 loc from to val released ord
+      (WF: Configuration.wf c1)
+      (STEP: small_step withprm tid e c1 c2)
+      (WRITING: ThreadEvent.is_writing e = Some (loc, from, to, val, released, ord)):
+  nonpromise c2 loc from to (Message.mk val released).
+Proof.
+  inv STEP. inv STEP0; inv STEP; inv WRITING.
+  - inv LOCAL. inv WRITE. inv PROMISE.
+    { econs; s.
+      - erewrite Memory.add_o; eauto. condtac; ss. des; congr.
+      - ii. inv H. revert TID0. rewrite IdentMap.gsspec. condtac.
+        + i. inv TID0. apply inj_pair2 in H1. subst. ss.
+          revert PROMISES0. erewrite Memory.remove_o; eauto. condtac; ss.
+          des; congr.
+        + i. exploit Memory.add_get0; eauto. i.
+          inv WF. inv WF0. exploit THREADS; eauto. i. inv x.
+          apply PROMISES1 in PROMISES0. congr.
+    }
+    { econs; s.
+      - erewrite Memory.split_o; eauto. condtac; ss.
+        exfalso. clear -o. des; apply o; auto.
+      - ii. inv H. revert TID0. rewrite IdentMap.gsspec. condtac.
+        + i. inv TID0. apply inj_pair2 in H1. subst. ss.
+          revert PROMISES0. erewrite Memory.remove_o; eauto. condtac; ss.
+          des; congr.
+        + i. exploit Memory.split_get0; eauto. i. des.
+          inv WF. inv WF0. exploit THREADS; eauto. i. inv x.
+          apply PROMISES1 in PROMISES0. congr.
+    }
+    { econs; s.
+      - erewrite Memory.lower_o; eauto. condtac; ss. des; congr.
+      - ii. inv H. revert TID0. rewrite IdentMap.gsspec. condtac.
+        + i. inv TID0. apply inj_pair2 in H1. subst. ss.
+          revert PROMISES0. erewrite Memory.remove_o; eauto. condtac; ss.
+          des; congr.
+        + i. exploit Memory.lower_get0; eauto. i.
+          inv WF. inv WF0. exploit DISJOINT; eauto. i.
+          eapply Memory.disjoint_get; try apply x; eauto.
+          eapply Memory.lower_get0. eauto.
+    }
+  - inv LOCAL1. clear GET.
+    inv LOCAL2. inv WRITE. inv PROMISE.
+    { econs; s.
+      - erewrite Memory.add_o; eauto. condtac; ss. des; congr.
+      - ii. inv H. revert TID0. rewrite IdentMap.gsspec. condtac.
+        + i. inv TID0. apply inj_pair2 in H1. subst. ss.
+          revert PROMISES0. erewrite Memory.remove_o; eauto. condtac; ss.
+          des; congr.
+        + i. exploit Memory.add_get0; eauto. i.
+          inv WF. inv WF0. exploit THREADS; eauto. i. inv x.
+          apply PROMISES1 in PROMISES0. congr.
+    }
+    { econs; s.
+      - erewrite Memory.split_o; eauto. condtac; ss.
+        exfalso. clear -o. des; apply o; auto.
+      - ii. inv H. revert TID0. rewrite IdentMap.gsspec. condtac.
+        + i. inv TID0. apply inj_pair2 in H1. subst. ss.
+          revert PROMISES0. erewrite Memory.remove_o; eauto. condtac; ss.
+          des; congr.
+        + i. exploit Memory.split_get0; eauto. i. des.
+          inv WF. inv WF0. exploit THREADS; eauto. i. inv x.
+          apply PROMISES1 in PROMISES0. congr.
+    }
+    { econs; s.
+      - erewrite Memory.lower_o; eauto. condtac; ss. des; congr.
+      - ii. inv H. revert TID0. rewrite IdentMap.gsspec. condtac.
+        + i. inv TID0. apply inj_pair2 in H1. subst. ss.
+          revert PROMISES0. erewrite Memory.remove_o; eauto. condtac; ss.
+          des; congr.
+        + i. exploit Memory.lower_get0; eauto. i.
+          inv WF. inv WF0. exploit DISJOINT; eauto. i.
+          eapply Memory.disjoint_get; try apply x; eauto.
+          eapply Memory.lower_get0. eauto.
+    }
+Qed.
+
+Lemma writing_small_step_nonpromise_backward
+      withprm tid e c1 c2 loc from to val released ord
+      (WF: Configuration.wf c1)
+      (STEP: small_step withprm tid e c1 c2)
+      (WRITING: ThreadEvent.is_writing e = Some (loc, from, to, val, released, ord)):
+  forall l f t msg
+    (NP: nonpromise c2 l f t msg),
+    nonpromise c1 l f t msg \/ (l, f, t, msg) = (loc, from, to, Message.mk val released).
+Proof.
+  inv STEP. inv STEP0; inv STEP; inv WRITING.
+  - inv LOCAL. inv WRITE. inv PROMISE.
+    { i. inv NP. ss. revert GET. erewrite Memory.add_o; eauto. condtac; ss.
+      { i. des. inv GET. auto. }
+      { left. econs; eauto. ii. inv H.
+        destruct (Ident.eq_dec tid0 tid).
+        - subst. rewrite TID in TID0. inv TID0. apply inj_pair2 in H1. subst.
+          eapply NONPROMISE. econs.
+          + rewrite IdentMap.gss. eauto.
+          + s. erewrite Memory.remove_o; eauto. condtac; ss.
+            erewrite Memory.add_o; eauto. condtac; [|eauto]. ss.
+        - eapply NONPROMISE. econs; eauto.
+          rewrite IdentMap.gso; eauto.
+      }
+    }
+    { i. inv NP. ss. revert GET. erewrite Memory.split_o; eauto. condtac; ss.
+      { i. des. inv GET. auto. }
+      guardH o. condtac; ss.
+      { i. des. inv GET. exfalso. eapply NONPROMISE. econs.
+        - rewrite IdentMap.gss. eauto.
+        - erewrite Memory.remove_o; eauto. condtac; ss.
+          erewrite Memory.split_o; eauto.
+          do 2 (condtac; try congr). eauto.
+      }
+      { left. econs; eauto. ii. inv H.
+        destruct (Ident.eq_dec tid0 tid).
+        - subst. rewrite TID in TID0. inv TID0. apply inj_pair2 in H1. subst.
+          eapply NONPROMISE. econs.
+          + rewrite IdentMap.gss. eauto.
+          + s. erewrite Memory.remove_o; eauto. condtac; ss.
+            erewrite Memory.split_o; eauto. do 2 (condtac; try congr). eauto.
+        - eapply NONPROMISE. econs; eauto.
+          rewrite IdentMap.gso; eauto.
+      }
+    }
+    { i. inv NP. ss. revert GET. erewrite Memory.lower_o; eauto. condtac; ss.
+      { i. des. inv GET. auto. }
+      { left. econs; eauto. ii. inv H.
+        destruct (Ident.eq_dec tid0 tid).
+        - subst. rewrite TID in TID0. inv TID0. apply inj_pair2 in H1. subst.
+          eapply NONPROMISE. econs.
+          + rewrite IdentMap.gss. eauto.
+          + s. erewrite Memory.remove_o; eauto. condtac; ss.
+            erewrite Memory.lower_o; eauto. condtac; [|eauto]. ss.
+        - eapply NONPROMISE. econs; eauto.
+          rewrite IdentMap.gso; eauto.
+      }
+    }
+  - inv LOCAL1. clear GET.
+    inv LOCAL2. inv WRITE. inv PROMISE.
+    { i. inv NP. ss. revert GET. erewrite Memory.add_o; eauto. condtac; ss.
+      { i. des. inv GET. auto. }
+      { left. econs; eauto. ii. inv H.
+        destruct (Ident.eq_dec tid0 tid).
+        - subst. rewrite TID in TID0. inv TID0. apply inj_pair2 in H1. subst.
+          eapply NONPROMISE. econs.
+          + rewrite IdentMap.gss. eauto.
+          + s. erewrite Memory.remove_o; eauto. condtac; ss.
+            erewrite Memory.add_o; eauto. condtac; [|eauto]. ss.
+        - eapply NONPROMISE. econs; eauto.
+          rewrite IdentMap.gso; eauto.
+      }
+    }
+    { i. inv NP. ss. revert GET. erewrite Memory.split_o; eauto. condtac; ss.
+      { i. des. inv GET. auto. }
+      guardH o. condtac; ss.
+      { i. des. inv GET. exfalso. eapply NONPROMISE. econs.
+        - rewrite IdentMap.gss. eauto.
+        - erewrite Memory.remove_o; eauto. condtac; ss.
+          erewrite Memory.split_o; eauto.
+          do 2 (condtac; try congr). eauto.
+      }
+      { left. econs; eauto. ii. inv H.
+        destruct (Ident.eq_dec tid0 tid).
+        - subst. rewrite TID in TID0. inv TID0. apply inj_pair2 in H1. subst.
+          eapply NONPROMISE. econs.
+          + rewrite IdentMap.gss. eauto.
+          + s. erewrite Memory.remove_o; eauto. condtac; ss.
+            erewrite Memory.split_o; eauto. do 2 (condtac; try congr). eauto.
+        - eapply NONPROMISE. econs; eauto.
+          rewrite IdentMap.gso; eauto.
+      }
+    }
+    { i. inv NP. ss. revert GET. erewrite Memory.lower_o; eauto. condtac; ss.
+      { i. des. inv GET. auto. }
+      { left. econs; eauto. ii. inv H.
+        destruct (Ident.eq_dec tid0 tid).
+        - subst. rewrite TID in TID0. inv TID0. apply inj_pair2 in H1. subst.
+          eapply NONPROMISE. econs.
+          + rewrite IdentMap.gss. eauto.
+          + s. erewrite Memory.remove_o; eauto. condtac; ss.
+            erewrite Memory.lower_o; eauto. condtac; [|eauto]. ss.
+        - eapply NONPROMISE. econs; eauto.
+          rewrite IdentMap.gso; eauto.
+      }
+    }
+Qed.
+
+Lemma writing_small_step_nonpromise
+      withprm tid e c1 c2 loc from to val released ord
+      (WF: Configuration.wf c1)
+      (STEP: small_step withprm tid e c1 c2)
+      (WRITING: ThreadEvent.is_writing e = Some (loc, from, to, val, released, ord)):
+  forall l f t msg,
+    nonpromise c2 l f t msg <-> nonpromise c1 l f t msg \/ (l, f, t, msg) = (loc, from, to, Message.mk val released).
+Proof.
+  econs; i.
+  - eapply writing_small_step_nonpromise_backward; eauto.
+  - des.
+    + eapply writing_small_step_nonpromise_forward; eauto.
+    + inv H. eapply writing_small_step_nonpromise_new; eauto.
+Qed.
